@@ -1,0 +1,92 @@
+module
+
+public import Roolean.QfBv.BvTerm
+public import Roolean.SmtLib2.Lexer
+
+public inductive Proof.SmtNode
+  | Relevant
+  | Irrelevant
+  | Split (varIndex: Nat) (bitIndex: Nat)
+    (left: SmtNode) (right: SmtNode)
+
+
+public structure SmtProof where
+  result: Bool
+  root: Proof.SmtNode
+
+namespace Proof
+
+public inductive ParserError
+  | ExpectedProof
+  | ExpectedProofResult
+  | ExpectedNode
+  | ExpectedParenOpen
+  | ExpectedParenClose
+deriving Repr, Nonempty, Inhabited
+
+public structure Parser where
+  tokens: List Token
+  initial: List Token
+deriving Repr, Nonempty, Inhabited
+
+public inductive EParser where
+  | Lexer (err: ELexer)
+  | Parser (err: ParserError) (parser: Parser)
+deriving Repr, Nonempty, Inhabited
+
+def Parser.error (parser: Parser) (err: ParserError) : EParser :=
+  EParser.Parser err parser
+
+def Parser.with (parser: Parser) (tokens: List Token) : Parser :=
+  { tokens := tokens, initial := parser.initial }
+
+def consumeParenClose(parser: Parser): Except EParser (Parser) :=
+  match parser.tokens with
+  | Token.ParenClose :: tokens => pure (parser.with tokens)
+  | _ => Except.error (parser.error ParserError.ExpectedParenClose)
+
+partial def parseNode (parser: Parser) : Except EParser (Parser × SmtNode) := do
+  match parser.tokens with
+    | Token.Symbol name :: tokens =>
+      match name.toString? with
+      | some "relevant" => pure (parser.with tokens, SmtNode.Relevant)
+      | some "irrelevant" => pure (parser.with tokens, SmtNode.Irrelevant)
+      | _ => Except.error (parser.error ParserError.ExpectedNode)
+
+    | Token.ParenOpen :: Token.Symbol name ::
+      Token.Numeral varIndex _ :: Token.Numeral bitIndex _ :: tokens =>
+      match name.toString? with
+      | some "decision" =>
+        let (parser, left) ← parseNode (parser.with tokens)
+        let (parser, right) ← parseNode parser
+        let parser ← consumeParenClose parser
+        pure (parser, SmtNode.Split varIndex bitIndex left right)
+
+      | _ => Except.error (parser.error ParserError.ExpectedNode)
+    | _ => Except.error (parser.error ParserError.ExpectedNode)
+
+
+partial def parseProof (parser: Parser) : Except EParser SmtProof := do
+  match parser.tokens with
+    | Token.ParenOpen :: Token.Symbol name :: Token.Symbol result :: tokens =>
+      let _ ← match name.toString? with
+        | "roole-proof" => pure ()
+        | _ => Except.error (parser.error ParserError.ExpectedProof)
+
+      let result ← match result.toString? with
+        | some "true" => pure true
+        | some "false" => pure false
+        | _ => Except.error (parser.error ParserError.ExpectedProofResult)
+      let (parser, root) ← parseNode (parser.with tokens)
+      let _ ← consumeParenClose parser
+      pure { result, root }
+    | _ => Except.error (parser.error ParserError.ExpectedProof)
+
+public def parse (chars: List Char8): Except EParser SmtProof :=
+  match lex chars with
+    | Except.ok tokens => do
+      let tokens := tokens.toList
+      let parser : Parser := { tokens, initial := tokens }
+      let parsed ← parseProof parser
+      pure parsed
+    | Except.error err => Except.error (EParser.Lexer err)
